zoo_parabs/algo: Verify [fold].

lib/zoo_parabs/algo.ml
@@ -36,7 +36,8 @@ let rec fold_seq ctx beg end_ body op acc =
   if beg == end_ then
     acc
   else
-    let acc = op acc (body ctx beg) in
+    let v = body ctx beg in
+    let acc = op acc v in
     let beg = beg + 1 in
     fold_seq ctx beg end_ body op acc
 let rec fold ctx beg end_ chunk body op zero =
