theories/zoo/prelude.v
@@ -20,3 +20,25 @@ Notation "⁺ n" := (
   right associativity,
   format "⁺ n"
 ) : stdpp_scope.
+
+Reserved Notation "x0 ≤ x1 ≤ x2 ≤ x3 ≤ x4"
+( at level 70,
+  x1 at next level,
+  x2 at next level,
+  x3 at next level,
+  x4 at next level
+).
+Notation "x0 ≤ x1 ≤ x2 ≤ x3 ≤ x4" := (
+  x0 ≤ x1 ∧
+  x1 ≤ x2 ∧
+  x2 ≤ x3 ∧
+  x3 ≤ x4
+)%nat
+: nat_scope.
+Notation "x0 ≤ x1 ≤ x2 ≤ x3 ≤ x4" := (
+  x0 ≤ x1 ∧
+  x1 ≤ x2 ∧
+  x2 ≤ x3 ∧
+  x3 ≤ x4
+)%Z
+: Z_scope.
